Make things importable by splitting main from lib part.
Also attempt lint checks in lean metaprogramming, but it's ugly, error
messages are ugly, and I need to check further it works.

solvers/1.lean
@@ -1,19 +1,5 @@
-import ProjectEulerStatements.P1
+import ProjectEulerSolutions.P1
 
-namespace ProjectEulerSolutions.P1
-
-def sumOfMultiples (m n : Nat) : Nat :=
-  let k := n / m
-  (m * k * (k + 1)) / 2
-
-def solve (n : Nat) : Nat :=
-  let n' := n - 1
-  sumOfMultiples 3 n' + sumOfMultiples 5 n' - sumOfMultiples 15 n'
-
-example : solve 10 = 23 := rfl
-theorem equiv (n : Nat) : ProjectEulerStatements.P1.naive n = solve n := sorry
-
-end ProjectEulerSolutions.P1
 open ProjectEulerSolutions.P1
 
 def main : IO Unit := do
