solvers/20.lean
@@ -1,23 +1,5 @@
-import ProjectEulerStatements.P20
-namespace ProjectEulerSolutions.P20
+import ProjectEulerSolutions.P20
 
-partial def digitSum (n : Nat) : Nat :=
-  let s := toString n
-  s.data.foldl (fun acc c => acc + (c.toNat - '0'.toNat)) 0
-
-partial def solve (n : Nat) : Nat :=
-  let rec loop (k acc : Nat) : Nat :=
-    if k > n then
-      digitSum acc
-    else
-      loop (k + 1) (acc * k)
-  loop 2 1
-
-example : solve 10 = 27 := by
-  native_decide
-
-theorem equiv (n : Nat) : ProjectEulerStatements.P20.naive n = solve n := sorry
-end ProjectEulerSolutions.P20
 open ProjectEulerSolutions.P20
 
 def main : IO Unit := do
