solvers/29.lean
@@ -1,31 +1,5 @@
-import ProjectEulerStatements.P29
-namespace ProjectEulerSolutions.P29
+import ProjectEulerSolutions.P29
 
-partial def countDistinctPowers (maxA maxB : Nat) : Nat :=
-  let rec loopA (a : Nat) (vals : List Nat) : List Nat :=
-    if a > maxA then
-      vals
-    else
-      let rec loopB (b : Nat) (vals : List Nat) : List Nat :=
-        if b > maxB then
-          vals
-        else
-          let v := a ^ b
-          let vals' := if vals.contains v then vals else v :: vals
-          loopB (b + 1) vals'
-      loopA (a + 1) (loopB 2 vals)
-  (loopA 2 []).length
-
-
-example : countDistinctPowers 5 5 = 15 := by
-  native_decide
-
-
-def solve (_n : Nat) : Nat :=
-  countDistinctPowers 100 100
-
-theorem equiv (n : Nat) : ProjectEulerStatements.P29.naive n n = solve n := sorry
-end ProjectEulerSolutions.P29
 open ProjectEulerSolutions.P29
 
 def main : IO Unit := do
