solvers/3.lean
@@ -1,32 +1,5 @@
-import ProjectEulerStatements.P3
-namespace ProjectEulerSolutions.P3
+import ProjectEulerSolutions.P3
 
-partial def stripTwos (n : Nat) (largest : Nat) : Nat × Nat :=
-  if n % 2 == 0 then
-    stripTwos (n / 2) 2
-  else
-    (n, largest)
-
-partial def oddLoop (n f largest : Nat) : Nat :=
-  if f * f <= n then
-    if n % f == 0 then
-      oddLoop (n / f) f f
-    else
-      oddLoop n (f + 2) largest
-  else
-    if n > 1 then n else largest
-
-def solve (n : ProjectEulerStatements.P3.NatGE2) : Nat :=
-  let (n', largest') := stripTwos n.1 1
-  oddLoop n' 3 largest'
-
-example : solve ⟨13195, by decide⟩ = 29 := by
-  native_decide
-
-theorem equiv (n : ProjectEulerStatements.P3.NatGE2) :
-    ProjectEulerStatements.P3.naive n = solve n := sorry
-
-end ProjectEulerSolutions.P3
 open ProjectEulerSolutions.P3
 
 def main : IO Unit := do
