solvers/53.lean
@@ -1,33 +1,5 @@
-import ProjectEulerStatements.P53
-namespace ProjectEulerSolutions.P53
+import ProjectEulerSolutions.P53
 
-partial def countCombinatoricSelections (limitN threshold : Nat) : Nat :=
-  let rec loopN (n : Nat) (total : Nat) : Nat :=
-    if n > limitN then
-      total
-    else
-      let rec loopR (r : Nat) (c : Nat) (total : Nat) : Nat :=
-        if r > n / 2 then
-          loopN (n + 1) total
-        else
-          let c := c * (n - r + 1) / r
-          if c > threshold then
-            let total := total + (n - 2 * r + 1)
-            loopN (n + 1) total
-          else
-            loopR (r + 1) c total
-      loopR 1 1 total
-  loopN 1 0
-
-
-
-def solve (limitN threshold : Nat) :=
-  countCombinatoricSelections limitN threshold
-
-theorem equiv (limitN threshold : Nat) :
-    ProjectEulerStatements.P53.naive limitN threshold = solve limitN threshold := sorry
-
-end ProjectEulerSolutions.P53
 open ProjectEulerSolutions.P53
 
 def main : IO Unit := do
