solvers/76.lean
@@ -1,33 +1,5 @@
-import ProjectEulerStatements.P76
-namespace ProjectEulerSolutions.P76
+import ProjectEulerSolutions.P76
 
-partial def countSummations (n : Nat) : Nat :=
-  let dp0 := Array.replicate (n + 1) 0
-  let dp0 := dp0.set! 0 1
-  let rec loopPart (part : Nat) (dp : Array Nat) : Array Nat :=
-    if part >= n then
-      dp
-    else
-      let rec loopS (s : Nat) (dp : Array Nat) : Array Nat :=
-        if s > n then
-          dp
-        else
-          let dp := dp.set! s (dp[s]! + dp[s - part]!)
-          loopS (s + 1) dp
-      loopPart (part + 1) (loopS part dp)
-  let dp := loopPart 1 dp0
-  dp[n]!
-
-
-example : countSummations 5 = 6 := by
-  native_decide
-
-
-def solve (_n : Nat) :=
-  countSummations 100
-
-theorem equiv (n : Nat) : ProjectEulerStatements.P76.naive n = solve n := sorry
-end ProjectEulerSolutions.P76
 open ProjectEulerSolutions.P76
 
 def main : IO Unit := do
