ProjectEulerSolutions/P1.lean
@@ -1,0 +1,16 @@
+import ProjectEulerStatements.P1
+
+namespace ProjectEulerSolutions.P1
+
+def sumOfMultiples (m n : Nat) : Nat :=
+  let k := n / m
+  (m * k * (k + 1)) / 2
+
+def solve (n : Nat) : Nat :=
+  let n' := n - 1
+  sumOfMultiples 3 n' + sumOfMultiples 5 n' - sumOfMultiples 15 n'
+
+example : solve 10 = 23 := rfl
+theorem equiv (n : Nat) : ProjectEulerStatements.P1.naive n = solve n := sorry
+
+end ProjectEulerSolutions.P1
