ProjectEulerSolutions/P16.lean
@@ -1,0 +1,17 @@
+import ProjectEulerStatements.P16
+namespace ProjectEulerSolutions.P16
+
+partial def digitSum (n : Nat) : Nat :=
+  let s := toString n
+  s.data.foldl (fun acc c => acc + (c.toNat - '0'.toNat)) 0
+
+
+example : digitSum (Nat.pow 2 15) = 26 := by
+  native_decide
+
+
+def solve (_n : Nat) :=
+  digitSum (Nat.pow 2 1000)
+
+theorem equiv (n : Nat) : ProjectEulerStatements.P16.naive n = solve n := sorry
+end ProjectEulerSolutions.P16
