ProjectEulerSolutions/P2.lean
@@ -1,0 +1,17 @@
+import ProjectEulerStatements.P2
+
+namespace ProjectEulerSolutions.P2
+
+partial def solve (limit : Nat) : Nat :=
+  let rec go (a b total : Nat) : Nat :=
+    if a ≤ limit then
+      let total' := if a % 2 = 0 then total + a else total
+      go b (a + b) total'
+    else
+      total
+  go 1 2 0
+
+example : solve 4000000 = 4613732 := by native_decide
+theorem equiv (n : Nat) : ProjectEulerStatements.P2.naive n = solve n := sorry
+
+end ProjectEulerSolutions.P2
