ProjectEulerSolutions/P20.lean
@@ -1,0 +1,20 @@
+import ProjectEulerStatements.P20
+namespace ProjectEulerSolutions.P20
+
+partial def digitSum (n : Nat) : Nat :=
+  let s := toString n
+  s.data.foldl (fun acc c => acc + (c.toNat - '0'.toNat)) 0
+
+partial def solve (n : Nat) : Nat :=
+  let rec loop (k acc : Nat) : Nat :=
+    if k > n then
+      digitSum acc
+    else
+      loop (k + 1) (acc * k)
+  loop 2 1
+
+example : solve 10 = 27 := by
+  native_decide
+
+theorem equiv (n : Nat) : ProjectEulerStatements.P20.naive n = solve n := sorry
+end ProjectEulerSolutions.P20
