ProjectEulerSolutions/P4.lean
@@ -1,0 +1,43 @@
+import ProjectEulerStatements.P4
+namespace ProjectEulerSolutions.P4
+
+def isPalindrome (n : Nat) : Bool :=
+  let s := toString n
+  s = String.mk s.data.reverse
+
+partial def loopB (a b lo best bestA bestB : Nat) : Nat × Nat × Nat :=
+  if b < lo then
+    (best, bestA, bestB)
+  else
+    let prod := a * b
+    if prod <= best then
+      (best, bestA, bestB)
+    else if isPalindrome prod then
+      (prod, a, b)
+    else
+      loopB a (b - 1) lo best bestA bestB
+
+partial def loopA (a lo hi best bestA bestB : Nat) : Nat × Nat × Nat :=
+  if a < lo then
+    (best, bestA, bestB)
+  else if a * hi < best then
+    (best, bestA, bestB)
+  else
+    let (best', bestA', bestB') := loopB a a lo best bestA bestB
+    if a = 0 then
+      (best', bestA', bestB')
+    else
+      loopA (a - 1) lo hi best' bestA' bestB'
+
+def largestPalindromeProduct (lo hi : Nat) : Nat × Nat × Nat :=
+  loopA hi lo hi 0 0 0
+
+example : (largestPalindromeProduct 10 99).1 = 9009 := by
+  native_decide
+
+
+def solve (_n : Nat) : Nat :=
+  (largestPalindromeProduct 100 999).1
+
+theorem equiv (n : Nat) : ProjectEulerStatements.P4.naive n = solve n := sorry
+end ProjectEulerSolutions.P4
