ProjectEulerSolutions/P65.lean
@@ -1,0 +1,43 @@
+import ProjectEulerStatements.P65
+namespace ProjectEulerSolutions.P65
+
+partial def eContinuedFractionCoeffs (n : Nat) : List Nat :=
+  let rec loop (i : Nat) (acc : List Nat) : List Nat :=
+    if i >= n then
+      acc.reverse
+    else
+      let a := if i == 0 then 2 else if i % 3 == 2 then 2 * (i / 3 + 1) else 1
+      loop (i + 1) (a :: acc)
+  loop 0 []
+
+partial def convergentNumeratorDenominator (coeffs : List Nat) : Nat × Nat :=
+  let rec loop (cs : List Nat) (p_nm2 p_nm1 q_nm2 q_nm1 : Nat) : Nat × Nat :=
+    match cs with
+    | [] => (p_nm1, q_nm1)
+    | a :: cs =>
+        let p := a * p_nm1 + p_nm2
+        let q := a * q_nm1 + q_nm2
+        loop cs p_nm1 p q_nm1 q
+  loop coeffs 0 1 1 0
+
+partial def digitSum (x : Nat) : Nat :=
+  (toString x).data.foldl (fun acc c => acc + (c.toNat - '0'.toNat)) 0
+
+partial def solve (n : Nat) : Nat :=
+  let coeffs := eContinuedFractionCoeffs n
+  let p := (convergentNumeratorDenominator coeffs).1
+  digitSum p
+
+
+example :
+    let coeffs10 := eContinuedFractionCoeffs 10
+    let pq := convergentNumeratorDenominator coeffs10
+    pq = (1457, 536) := by
+  native_decide
+
+example : digitSum 1457 = 17 := by
+  native_decide
+
+
+theorem equiv (n : Nat) : ProjectEulerStatements.P65.naive n = solve n := sorry
+end ProjectEulerSolutions.P65
