ProjectEulerSolutions/P7.lean
@@ -1,0 +1,40 @@
+import ProjectEulerStatements.P7
+namespace ProjectEulerSolutions.P7
+
+partial def isPrimeWith (n : Nat) (primes : Array Nat) : Bool :=
+  let rec loop (i : Nat) : Bool :=
+    if i >= primes.size then
+      true
+    else
+      let p := primes[i]!
+      if p * p > n then
+        true
+      else if n % p == 0 then
+        false
+      else
+        loop (i + 1)
+  loop 0
+
+partial def solve (n : Nat) : Nat :=
+  if n == 1 then
+    2
+  else
+    let rec go (candidate count : Nat) (primes : Array Nat) : Nat :=
+      if count == n then
+        primes[primes.size - 1]!
+      else
+        if isPrimeWith candidate primes then
+          let primes' := primes.push candidate
+          go (candidate + 2) (count + 1) primes'
+        else
+          go (candidate + 2) count primes
+    go 3 1 #[2]
+
+example : solve 1 = 2 := by
+  native_decide
+
+example : solve 6 = 13 := by
+  native_decide
+
+theorem equiv (n : Nat) : ProjectEulerStatements.P7.naive n = solve n := sorry
+end ProjectEulerSolutions.P7
