ProjectEulerSolutions/P71.lean
@@ -1,0 +1,32 @@
+import ProjectEulerStatements.P71
+namespace ProjectEulerSolutions.P71
+
+partial def gcd (a b : Nat) : Nat :=
+  if b == 0 then a else gcd b (a % b)
+
+partial def bestFractionLeftOf (targetN targetD maxD : Nat) : Nat × Nat :=
+  let rec loop (d : Nat) (bestN bestD : Nat) : Nat × Nat :=
+    if d > maxD then
+      (bestN, bestD)
+    else
+      let n := (targetN * d - 1) / targetD
+      if n == 0 then
+        loop (d + 1) bestN bestD
+      else if gcd n d != 1 then
+        loop (d + 1) bestN bestD
+      else if n * bestD > bestN * d then
+        loop (d + 1) n d
+      else
+        loop (d + 1) bestN bestD
+  loop 1 0 1
+
+
+example : bestFractionLeftOf 3 7 8 = (2, 5) := by
+  native_decide
+
+
+def solve (_n : Nat) :=
+  (bestFractionLeftOf 3 7 1000000).1
+
+theorem equiv (n : Nat) : ProjectEulerStatements.P71.naive n = solve n := sorry
+end ProjectEulerSolutions.P71
