ProjectEulerSolutions/P91.lean
@@ -1,0 +1,40 @@
+import ProjectEulerStatements.P91
+namespace ProjectEulerSolutions.P91
+
+partial def gcd (a b : Nat) : Nat :=
+  if b == 0 then a else gcd b (a % b)
+
+partial def countRightTriangles (n : Nat) : Nat :=
+  let total := n * n
+  let rec loopX (x : Nat) (acc : Nat) : Nat :=
+    if x > n then
+      acc
+    else
+      let rec loopY (y : Nat) (acc : Nat) : Nat :=
+        if y > n then
+          acc
+        else
+          if x == 0 && y == 0 then
+            loopY (y + 1) acc
+          else if x == 0 || y == 0 then
+            loopY (y + 1) (acc + n)
+          else
+            let g := gcd x y
+            let dx := y / g
+            let dy := x / g
+            let k1 := Nat.min (x / dx) ((n - y) / dy)
+            let k2 := Nat.min ((n - x) / dx) (y / dy)
+            loopY (y + 1) (acc + k1 + k2)
+      loopX (x + 1) (loopY 0 acc)
+  loopX 0 total
+
+
+example : countRightTriangles 2 = 14 := by
+  native_decide
+
+
+def solve (_n : Nat) :=
+  countRightTriangles 50
+
+theorem equiv (n : Nat) : ProjectEulerStatements.P91.naive n = solve n := sorry
+end ProjectEulerSolutions.P91
